Add removeNode and addNodeN operations to gfg API
Also extend wfg predicate to require well-formedness of the underlying
sptree values. There still needs one further condition added: that the
corresponding predecessor and follower maps contain the same
information.

examples/generic_finite_graphs/gfgScript.sml
@@ -55,37 +55,36 @@ val wfAdjacency_def = Define‘
      ∀k nl e n. lookup k adjmap = SOME nl ∧ MEM (e,n) nl ⇒
                 n ∈ domain adjmap’;
 
-val wfg_def = Define‘
+Definition wfg_def:
   wfg g ⇔ (∀n. g.next ≤ n ⇒ n ∉ domain g.nodeInfo) ∧
            (domain g.followers = domain g.nodeInfo) ∧
            (domain g.preds = domain g.nodeInfo) ∧
-           wfAdjacency g.followers ∧ wfAdjacency g.preds’;
+           wf g.nodeInfo ∧ wf g.followers ∧ wf g.preds ∧
+           wfAdjacency g.followers ∧ wfAdjacency g.preds
+End
 
-val empty_is_wfg = Q.store_thm(
-  "empty_is_wfg[simp]",
-  `wfg empty`,
-  simp[empty_def,wfg_def,wfAdjacency_def] >> rpt strip_tac
-  >> fs[lookup_def]
-    );
+Theorem empty_is_wfg[simp]:
+  wfg empty
+Proof
+  simp[empty_def,wfg_def,wfAdjacency_def] >> rpt strip_tac >> fs[lookup_def]
+QED
 
-val cond_eq = Q.prove(
-  ‘((if P then t else e) = v) ⇔ P ∧ t = v ∨ ¬P ∧ e = v’,
-  rw[]);
-
-val addNode_preserves_wfg = Q.store_thm(
-  "addNode_preserves_wfg[simp]",
-  ‘wfg g ⇒ wfg (addNode i g)’,
-  simp[wfg_def, addNode_def] >>
-  dsimp[wfAdjacency_def, lookup_insert, cond_eq] >> metis_tac[]);
+Theorem addNode_preserves_wfg[simp]:
+  wfg g ⇒ wfg (addNode i g)
+Proof
+  simp[wfg_def, addNode_def, sptreeTheory.wf_insert] >>
+  dsimp[wfAdjacency_def, lookup_insert, AllCaseEqs()] >> metis_tac[]
+QED
 
 Theorem addEdge_preserves_wfg:
   wfg g ∧ (addEdge i (e,s) g = SOME g2) ==> wfg g2
 Proof
   simp[wfg_def,addEdge_def] >>
-  dsimp[wfAdjacency_def, lookup_insert] >> rpt strip_tac >> rw[] >> fs[]
+  dsimp[wfAdjacency_def, lookup_insert] >> rpt strip_tac >> rw[] >>
+  fs[sptreeTheory.wf_insert] >>
+  drule_then strip_assume_tac (SRULE [PULL_EXISTS] $ iffRL domain_lookup) >>
+  simp[ABSORPTION_RWT]
   >- metis_tac[]
-  >- (fs[INSERT_DEF,SET_EQ_SUBSET,SUBSET_DEF] >> rpt strip_tac >> metis_tac[])
-  >- (fs[INSERT_DEF,SET_EQ_SUBSET,SUBSET_DEF] >> rpt strip_tac >> metis_tac[])
   >- (rename[`lookup k (insert i _ _) = SOME nl`, `MEM (e',n) nl`,
              ‘i ∈ domain _’] >>
       fs[lookup_insert] >> Cases_on `k=i` >> fs[] >>
@@ -103,14 +102,12 @@ val addEdge_preserves_nodeInfo = Q.store_thm(
    rpt strip_tac >> fs[addEdge_def,theorem "gfg_component_equality"]
     );
 
-val updateNode_preserves_wfg = Q.store_thm(
-   "updateNode_preserves_wfg[simp]",
-   `wfg g ∧ (updateNode id n g = SOME g2) ==> wfg g2`,
-   simp[wfg_def,updateNode_def]
-   >> dsimp[wfAdjacency_def, lookup_insert]
-   >> rw[] >> fs[INSERT_DEF,SET_EQ_SUBSET,SUBSET_DEF]
-   >> rpt strip_tac >> metis_tac[]
-    );
+Theorem updateNode_preserves_wfg[simp]:
+  wfg g ∧ (updateNode id n g = SOME g2) ==> wfg g2
+Proof
+   simp[wfg_def,updateNode_def] >> rw[] >> simp[] >>
+   gs[ABSORPTION_RWT, wf_insert] >> metis_tac[]
+QED
 
 val updateNode_preserves_edges = Q.store_thm(
     "updateNode_preserves_edges",
@@ -136,5 +133,84 @@ val graph_size_addNode = Q.store_thm(
   "graph_size_addNode[simp]",
   ‘wfg g ⇒ graph_size (addNode i g) = graph_size g + 1’,
   simp[graph_size_def, addNode_def, size_insert, wfg_def]);
+
+Definition removeEdges_on_def:
+  removeEdges_on n g =
+  if n ∈ domain g.nodeInfo then
+  g with <|
+      followers updated_by (insert n [] o map (FILTER (λei. SND ei ≠ n))) ;
+      preds updated_by (insert n [] o map (FILTER (λei. SND ei ≠ n))) ;
+    |>
+  else g
+End
+
+Theorem removeEdges_on_preserves_wfg:
+  wfg g ⇒ wfg (removeEdges_on n g)
+Proof
+  rw[wfg_def, removeEdges_on_def, sptreeTheory.domain_map,
+     pred_setTheory.ABSORPTION_RWT, wf_insert] >>
+  gs[wfAdjacency_def, sptreeTheory.domain_map] >>
+  rw[sptreeTheory.lookup_insert] >>
+  gs[sptreeTheory.lookup_map, listTheory.MEM_FILTER] >> metis_tac[]
+QED
+
+Theorem removeEdges_on_next[simp]:
+  (removeEdges_on n g).next = g.next
+Proof
+  rw[removeEdges_on_def]
+QED
+
+Theorem domain_removeEdges_on:
+  wfg g ⇒
+  domain (removeEdges_on n g).nodeInfo = domain g.nodeInfo ∧
+  domain (removeEdges_on n g).followers = domain g.followers ∧
+  domain (removeEdges_on n g).preds = domain g.preds
+Proof
+  rw[removeEdges_on_def, sptreeTheory.domain_map, pred_setTheory.ABSORPTION_RWT,
+     wfg_def]
+QED
+
+Definition deleteNode_def:
+  deleteNode n g = removeEdges_on n g with <|
+                                    nodeInfo updated_by (delete n) ;
+                                    followers updated_by (delete n) ;
+                                    preds updated_by (delete n)
+                                  |>
+End
+
+Theorem deleteNode_preserves_wfg:
+  wfg g ⇒ wfg (deleteNode n g)
+Proof
+  rw[deleteNode_def] >>
+  rw[wfg_def, domain_removeEdges_on] >>
+  gvs[wfg_def, wfAdjacency_def, sptreeTheory.lookup_delete,
+      removeEdges_on_def, wf_delete] >>
+  rw[] >>
+  gs[lookup_insert, lookup_map, wf_delete, wf_insert, domain_map, MEM_FILTER] >>
+  metis_tac[]
+QED
+
+Definition addNodeN_def:
+  addNodeN n i g =
+  if n ∈ domain g.nodeInfo then g with nodeInfo updated_by (insert n i)
+  else g with <| nodeInfo updated_by (insert n i);
+                 preds updated_by (insert n []) ;
+                 followers updated_by (insert n []);
+                 next := MAX g.next (n + 1) |>
+End
+
+Theorem addNodeN_preserves_wfg:
+  wfg g ⇒ wfg (addNodeN n i g)
+Proof
+  rw[wfg_def, addNodeN_def, ABSORPTION_RWT, wf_insert] >>
+  gs[wfAdjacency_def, sptreeTheory.lookup_insert, AllCaseEqs(),
+     ABSORPTION_RWT, SF DNF_ss] >> metis_tac[]
+QED
+
+Theorem nodes_addNodeN[simp]:
+  domain (addNodeN n i g).nodeInfo = n INSERT domain g.nodeInfo
+Proof
+  rw[addNodeN_def, pred_setTheory.ABSORPTION_RWT]
+QED
 
 val _ = export_theory();
